fix spec for dlist_ok

src/Dir.v
@@ -747,7 +747,10 @@ Module DIR.
     end.
 
 
-  Definition dlist_f (s : list (filename * addr)) (de : dent) := Eval compute_rec in
+  Definition dlistent := (filename * addr)%type.
+  Definition dlmatch (de: dlistent) : @pred _ (@weq filename_len) _ := fst de |-> snd de.
+
+  Definition dlist_f (s : list dlistent) (de : dent) := Eval compute_rec in
     if (weq (de :-> "valid") $0) then s
     else (de :-> "name", de :-> "inum") :: s.
 
@@ -755,16 +758,13 @@ Module DIR.
     let2 (mscs, r) <- dfold lxp bxp ixp dnum dlist_f nil mscs;
     rx (mscs, r).
 
-  Definition diritem := (filename * addr)%type.
-  Definition diritemmatch (de: diritem) : @pred _ (@weq filename_len) _ := fst de |-> snd de.
-
   Theorem dlist_ok : forall lxp bxp ixp dnum mscs,
     {< F A mbase m dmap,
     PRE      MEMLOG.rep lxp (ActiveTxn mbase m) mscs *
              [[ rep F A m bxp ixp dnum dmap ]]
     POST:(mscs',res)
              MEMLOG.rep lxp (ActiveTxn mbase m) mscs' *
-             [[ listpred diritemmatch res dmap ]]
+             [[ listpred dlmatch res dmap ]]
     CRASH    MEMLOG.log_intact lxp mbase
     >} dlist lxp bxp ixp dnum mscs.
   Proof.
